micro example compiles and runs in extracted cakeml using new Resolute data structures (Resolute_Formula, Resolute_Term, Resolute_Evidence, Resolute_Judgement)

src/Resolute_JSON.v
@@ -4,9 +4,11 @@ Require Import Resolute_Logic Resolute_Types ErrorStringConstants.
 Require Export JSON List Maps EqClass JSON_Core ID_Type.
 Import ListNotations ResultNotation.
 
-Definition STR_RESOLUTE_SUCCESS : string := "RESOLUTE_POLICY_CHECK".
-Definition STR_RESOLUTE_FORMULA : string := "RESOLUTE_FORMULA".
+Definition STR_RESOLUTE_SUCCESS  : string := "RESOLUTE_POLICY_CHECK".
+Definition STR_RESOLUTE_FORMULA  : string := "RESOLUTE_FORMULA".
 Definition STR_RESOLUTE_EVIDENCE : string := "RESOLUTE_EVIDENCE".
+Definition STR_RESOLUTE_JUDGEMENT : string := "RESOLUTE_JUDGEMENT".
+Definition STR_RESOLUTE_TERM     : string := "RESOLUTE_TERM".
 
 Definition STR_RESOLUTE : string := "RESOLUTE".
 Definition r_false_name_constant : string := "R_False".
@@ -19,6 +21,14 @@ Definition r_imp_name_constant : string := "R_Imp".
 Definition r_goal_e_name_constant : string := "R_Goal_E".
 Definition r_and_e_name_constant : string := "R_And_E".
 Definition r_or_e_name_constant : string := "R_Or_E".
+
+Definition r_goal_t_name_constant : string := "R_Goal_T".
+Definition r_and_t_name_constant : string := "R_And_T".
+Definition r_or_t_name_constant : string := "R_Or_T".
+
+Definition r_goal_j_name_constant : string := "R_Goal_J".
+Definition r_and_j_name_constant : string := "R_And_J".
+Definition r_or_j_name_constant : string := "R_Or_J".
 
 Fixpoint Resolute_to_JSON (t : Resolute_Formula)  : JSON := 
   match t with
@@ -135,6 +145,120 @@ Fixpoint Resolute_Evidence_from_JSON `{Jsonifiable Evidence} (js : JSON) : Resul
     | errC e => errC e
     end.
 
+Fixpoint Resolute_Term_to_JSON `{Jsonifiable Term} (t : Resolute_Term)  : JSON := 
+  match t with
+  | R_Goal_T tid args t => constructor_to_JSON STR_RESOLUTE_TERM r_goal_t_name_constant [JSON_String (to_string tid); (to_JSON args); (to_JSON t)]
+  | R_And_T t1 t2 => constructor_to_JSON STR_RESOLUTE_TERM r_and_t_name_constant
+  [(Resolute_Term_to_JSON t1); (Resolute_Term_to_JSON t2)]
+  | R_Or_T t1 t2 => constructor_to_JSON STR_RESOLUTE_TERM r_or_t_name_constant
+  [(Resolute_Term_to_JSON t1); (Resolute_Term_to_JSON t2)]
+  end.
+    
+Fixpoint Resolute_Term_from_JSON `{Jsonifiable Term} (js : JSON) : ResultT Resolute_Term string :=
+    let type_name := STR_RESOLUTE_TERM in
+    let type_str := type_name ++ type_sep ++ type_string_constant in
+    let body_str := type_name ++ type_sep ++ body_string_constant in
+    match (JSON_get_Object type_str js) with
+    | resultC (JSON_String cons_name) =>
+
+      if (eqb cons_name r_goal_t_name_constant) 
+      then 
+      match (JSON_get_Object body_str js) with 
+      | resultC (JSON_Array
+                  [(JSON_String n_js); args_js; t_js]) =>
+          n <- from_string n_js ;;
+          args <- from_JSON args_js ;;
+          t <- from_JSON t_js ;;
+          resultC (R_Goal_T n args t)
+        | _ => errC err_str_json_parsing_failure_wrong_number_args
+        end
+
+      else if (eqb cons_name r_and_t_name_constant) 
+      then match js with
+        | JSON_Object [
+            _;
+            (_, JSON_Array [ term1; term2 ])
+          ] =>
+            term1_val <- (Resolute_Term_from_JSON term1) ;;
+            term2_val <- (Resolute_Term_from_JSON term2) ;;
+            resultC (R_And_T term1_val term2_val)
+        | _ => errC err_str_json_parsing_failure_wrong_number_args
+        end
+
+      else if (eqb cons_name r_or_t_name_constant) 
+      then match js with
+        | JSON_Object [
+            _;
+            (_, JSON_Array [ term1; term2 ])
+          ] =>
+            term1_val <- (Resolute_Term_from_JSON term1) ;;
+            term2_val <- (Resolute_Term_from_JSON term2) ;;
+            resultC (R_Or_T term1_val term2_val)
+        | _ => errC err_str_json_parsing_failure_wrong_number_args
+        end
+
+      else errC err_str_json_invalid_constructor_name
+    | resultC _ => errC err_str_json_invalid_constructor_name
+    | errC e => errC e
+    end.
+
+Fixpoint Resolute_Judgement_to_JSON `{Jsonifiable bool} (t : Resolute_Judgement)  : JSON := 
+  match t with
+  | R_Goal_J tid args e => constructor_to_JSON STR_RESOLUTE_JUDGEMENT r_goal_j_name_constant [JSON_String (to_string tid); (to_JSON args); (to_JSON e)]
+  | R_And_J t1 t2 => constructor_to_JSON STR_RESOLUTE_JUDGEMENT r_and_j_name_constant
+  [(Resolute_Judgement_to_JSON t1); (Resolute_Judgement_to_JSON t2)]
+  | R_Or_J t1 t2 => constructor_to_JSON STR_RESOLUTE_JUDGEMENT r_or_j_name_constant
+  [(Resolute_Judgement_to_JSON t1); (Resolute_Judgement_to_JSON t2)]
+  end.
+        
+Fixpoint Resolute_Judgement_from_JSON `{Jsonifiable bool} (js : JSON) : ResultT Resolute_Judgement string :=
+    let type_name := STR_RESOLUTE_JUDGEMENT in
+    let type_str := type_name ++ type_sep ++ type_string_constant in
+    let body_str := type_name ++ type_sep ++ body_string_constant in
+    match (JSON_get_Object type_str js) with
+    | resultC (JSON_String cons_name) =>
+
+      if (eqb cons_name r_goal_j_name_constant) 
+      then 
+      match (JSON_get_Object body_str js) with 
+      | resultC (JSON_Array
+                  [(JSON_String n_js); args_js; jt_js]) =>
+          n <- from_string n_js ;;
+          args <- from_JSON args_js ;;
+          jt <- from_JSON jt_js ;;
+          resultC (R_Goal_J n args jt)
+        | _ => errC err_str_json_parsing_failure_wrong_number_args
+        end
+
+      else if (eqb cons_name r_and_j_name_constant) 
+      then match js with
+        | JSON_Object [
+            _;
+            (_, JSON_Array [ term1; term2 ])
+          ] =>
+            term1_val <- (Resolute_Judgement_from_JSON term1) ;;
+            term2_val <- (Resolute_Judgement_from_JSON term2) ;;
+            resultC (R_And_J term1_val term2_val)
+        | _ => errC err_str_json_parsing_failure_wrong_number_args
+        end
+
+      else if (eqb cons_name r_or_j_name_constant) 
+      then match js with
+        | JSON_Object [
+            _;
+            (_, JSON_Array [ term1; term2 ])
+          ] =>
+            term1_val <- (Resolute_Judgement_from_JSON term1) ;;
+            term2_val <- (Resolute_Judgement_from_JSON term2) ;;
+            resultC (R_Or_J term1_val term2_val)
+        | _ => errC err_str_json_parsing_failure_wrong_number_args
+        end
+
+      else errC err_str_json_invalid_constructor_name
+    | resultC _ => errC err_str_json_invalid_constructor_name
+    | errC e => errC e
+    end.
+
 Close Scope string_scope.
 
 Global Instance Jsonifiable_Resolute : Jsonifiable Resolute_Formula. 
@@ -144,36 +268,52 @@ repeat (result_monad_unfold;
 jsonifiable_hammer; repeat rewrite canonical_jsonification in *; eauto).
 Defined.
 
-Global Instance Jsonifiable_Resolute_Evidence : Jsonifiable Resolute_Evidence. 
+Global Instance Jsonifiable_Resolute_Evidence `{Jsonifiable Evidence} : Jsonifiable Resolute_Evidence. 
 eapply Build_Jsonifiable with (to_JSON := Resolute_Evidence_to_JSON) (from_JSON := Resolute_Evidence_from_JSON).
 induction a; 
 repeat (result_monad_unfold;
 jsonifiable_hammer; repeat rewrite canonical_jsonification in *; eauto).
 Defined.
 
-Definition ResoluteResponse_to_JSON `{Jsonifiable Term, Jsonifiable Resolute_Formula} (resp:ResoluteResponse) : JSON := 
+Global Instance Jsonifiable_Resolute_Term `{Jsonifiable Term} : Jsonifiable Resolute_Term. 
+eapply Build_Jsonifiable with (to_JSON := Resolute_Term_to_JSON) (from_JSON := Resolute_Term_from_JSON).
+induction a; 
+repeat (result_monad_unfold;
+jsonifiable_hammer; repeat rewrite canonical_jsonification in *; eauto).
+Defined.
+
+Global Instance Jsonifiable_Resolute_Judgement `{Jsonifiable bool} : Jsonifiable Resolute_Judgement. 
+eapply Build_Jsonifiable with (to_JSON := Resolute_Judgement_to_JSON) (from_JSON := Resolute_Judgement_from_JSON).
+induction a; 
+repeat (result_monad_unfold;
+jsonifiable_hammer; repeat rewrite canonical_jsonification in *; eauto).
+Defined.
+
+Definition ResoluteResponse_to_JSON `{Jsonifiable Resolute_Term, Jsonifiable Resolute_Formula, Jsonifiable Resolute_Judgement} (resp:ResoluteResponse) : JSON := 
 
   JSON_Object 
-    [(STR_RESOLUTE_SUCCESS, (JSON_Boolean (resoluteresp_success resp)));
+    [(STR_RESOLUTE_JUDGEMENT, (to_JSON (resoluteresp_judgement resp)));
     (STR_RESOLUTE_FORMULA, (to_JSON (resoluteresp_formula resp)));
-    (STR_TERM, (to_JSON (resoluteresp_term resp)))].
+    (STR_RESOLUTE_TERM, (to_JSON (resoluteresp_term resp)))].
 
-Definition ResoluteResponse_from_JSON `{Jsonifiable Term, Jsonifiable Resolute_Formula}
+Definition ResoluteResponse_from_JSON `{Jsonifiable Resolute_Term, Jsonifiable Resolute_Formula, Jsonifiable Resolute_Judgement}
 (resp:JSON) : ResultT ResoluteResponse string := 
-  temp_success <- JSON_get_bool STR_RESOLUTE_SUCCESS resp ;;
+  temp_success <- JSON_get_Object STR_RESOLUTE_JUDGEMENT resp ;;
   temp_formula <- JSON_get_Object STR_RESOLUTE_FORMULA resp ;;
-  temp_term <- JSON_get_Object STR_TERM resp ;;
+  temp_term <- JSON_get_Object STR_RESOLUTE_TERM resp ;;
 
+  judgement <- from_JSON temp_success ;;
   formula <- from_JSON temp_formula ;;
   term <- from_JSON temp_term ;;
-  resultC (mkResoluteResp temp_success formula term).
+  resultC (mkResoluteResp judgement formula term).
 
-
-Global Instance Jsonifiable_ResoluteResponse `{Jsonifiable Term, Jsonifiable Resolute_Formula}: Jsonifiable ResoluteResponse.
+Global Instance Jsonifiable_ResoluteResponse `{Jsonifiable Resolute_Judgement, Jsonifiable Resolute_Term, Jsonifiable Resolute_Formula}: Jsonifiable ResoluteResponse.
 eapply Build_Jsonifiable with
 (to_JSON := ResoluteResponse_to_JSON)
 (from_JSON := ResoluteResponse_from_JSON); unfold ResoluteResponse_to_JSON; unfold ResoluteResponse_from_JSON; solve_json.
 Defined.
 
-Definition test_resolute_resp_compute_json (x:ResoluteResponse) : JSON := to_JSON x.
+(*
+Definition test_resolute_resp_compute_json `{Jsonifiable ResoluteResponse} (x:ResoluteResponse) : JSON := to_JSON x.
+*)
 
