src/Resolute_Types.v
@@ -4,7 +4,7 @@ Require Import Term_Defs Resolute_Logic. (* Attestation_Session AppraisalSummary
 
 Record ResoluteResponse := 
     mkResoluteResp {
-      resoluteresp_success: bool;
+      resoluteresp_judgement: Resolute_Judgement;
       resoluteresp_formula: Resolute_Formula;
-      resoluteresp_term: Term;
+      resoluteresp_term: Resolute_Term;
   }.
